theories/Reductions/MM_to_MMA2.v
@@ -24,12 +24,86 @@ From Undecidability.Shared.Libs.DLW Require Import Utils.utils Vec.pos Vec.vec U
 From Undecidability.ILL.Code Require Import sss.
 From Undecidability.ILL.Mm Require Import mm_defs.
 From Undecidability.H10.Fractran Require Import fractran_defs prime_seq mm_fractran.
+From Undecidability.H10 Require Import MM_FRACTRAN.
 From Undecidability.MM Require Import mma_defs fractran_mma.
 
 Set Implicit Arguments.
 
 Local Notation "P /MM/ s ↓" := (sss_terminates (@mm_sss _) P s) (at level 70, no associativity). 
 Local Notation "P /MMA/ s ↓" := (sss_terminates (@mma_sss 2) P s) (at level 70, no associativity). 
+
+Theorem mm_fractran_reg n (P : list (mm_instr (pos n))) : 
+        { l : list (nat*nat) & { f |  Forall (fun c => snd c <> 0) l
+                                   /\ forall v, (1,P) /MM/ (1,v) ↓ <-> l /F/ f v ↓ } }.
+Proof.
+  destruct (mm_fractran_not_zero P) as (l & H1 & H2).
+  exists l, (fun v => ps 1 * exp 1 v); split; auto.
+  revert H1; apply Forall_impl; tauto.
+Qed.
+
+Section MM_FRACTRAN_REG.
+
+  Let f : MM_PROBLEM -> FRACTRAN_REG_PROBLEM.
+  Proof.
+    intros (n & P & v).
+    destruct (mm_fractran_reg P) as (l & f & H1 & H2).
+    exists l, (f v); assumption.
+  Defined.
+
+  Theorem MM_FRACTRAN_REG_HALTING : MM_HALTING ⪯ FRACTRAN_REG_HALTING.
+  Proof.
+    exists f. 
+    intros (n & P & v); simpl.
+    destruct (mm_fractran_reg P) as (l & g & H1 & H2); simpl; auto.
+  Qed.
+
+End MM_FRACTRAN_REG.
+
+Check MM_FRACTRAN_REG_HALTING.
+Print Assumptions MM_FRACTRAN_REG_HALTING.
+
+Theorem fractran_reg_mma2 l : 
+          Forall (fun c => snd c <> 0) l
+       ->   { Q : list (mm_instr (pos 2)) 
+            | forall x, l /F/ x ↓ <-> (1,Q) /MMA/ (1,x##0##vec_nil) ↓ }.
+Proof.
+  intros Hl.
+  exists (fractran_reg_mma l).
+  apply fractran_reg_mma_reduction; auto.
+Qed.
+
+Section FRACTRAN_REG_MMA2.
+
+  Let f : FRACTRAN_REG_PROBLEM -> MMA2_PROBLEM.
+  Proof.
+    intros (l & x & Hl).
+    destruct (fractran_reg_mma2 Hl) as (Q & HQ).
+    exact (Q, (x##0##vec_nil)).
+  Defined.
+
+  Theorem FRACTRAN_REG_MMA2_HALTING : FRACTRAN_REG_HALTING ⪯ MMA2_HALTING.
+  Proof.
+    exists f. 
+    intros (l & x & Hl); simpl.
+    destruct (fractran_reg_mma2 Hl) as (Q & HQ); apply HQ.
+  Qed.
+
+End FRACTRAN_REG_MMA2.
+
+Check FRACTRAN_REG_MMA2_HALTING.
+Print Assumptions FRACTRAN_REG_MMA2_HALTING.
+
+Corollary MM_MMA2_HALTING : MM_HALTING ⪯ MMA2_HALTING.
+Proof.
+  eapply reduces_transitive. exact MM_FRACTRAN_REG_HALTING.
+  exact FRACTRAN_REG_MMA2_HALTING.
+Qed.
+
+Check MM_MMA2_HALTING.
+Print Assumptions MM_MMA2_HALTING.
+
+(** This is somewhat for direct proof that does not involve
+    testing for (0,_) in the intermediate Fractran program *)
 
 Theorem mm_mma2 n (P : list (mm_instr (pos n))) : 
                {   Q : list (mm_instr (pos 2)) 
@@ -41,24 +115,3 @@ Proof.
   intros v; rewrite H2.
   apply fractran_mma_reduction; trivial.
 Qed.
-
-Section MM_MMA2.
-
-  Let f : MM_PROBLEM -> MMA2_PROBLEM.
-  Proof.
-    intros (n & P & v).
-    destruct (mm_mma2 P) as (Q & f & H).
-    exact (Q, f v).
-  Defined.
-
-  Theorem MM_MMA2_HALTING : MM_HALTING ⪯ MMA2_HALTING.
-  Proof.
-    exists f. 
-    intros (n & P & v); simpl; unfold MMA2_HALTING.
-    destruct (mm_mma2 P) as (Q & g & H); simpl; auto.
-  Qed.
-
-End MM_MMA2.
-
-Check MM_MMA2_HALTING.
-Print Assumptions MM_MMA2_HALTING.
